Versions/VOp.i.dfy
@@ -7,15 +7,58 @@ module VersionOp {
 
   type Loc = DiskLayout.Location
 
+  // StateViews lives side-by-side with JournalViews, together making
+  // up the CompositeViews, but in many ways, StateViews is subservient
+  // to JournalViews. JournalViews drives the syncing action,
+  // and furthermore, JournalViews is "incomplete" without StateViews
+  // (as its journals are meaningless without states to base them
+  // off of).
+
   datatype VOp =
-    | SendPersistentLocOp(loc: Loc)
-    | AdvanceOp(uiop: UI.Op, replay: bool)
-    | CrashOp
-    | FreezeOp
     | TristateInternalOp
     | JournalInternalOp
+
+    // This is where user-visible actions take place.
+    // On the StateViews, we advance the ephemeral state forward.
+    // From the JournalViews side, this might be replaying something
+    // from the journal or performing a new action.
+
+    | AdvanceOp(uiop: UI.Op, replay: bool)
+
+    // These describe the interaction between the StateViews
+    // and the JournalViews. The main interaction loop is, roughly:
+    //
+    // At initialization time, the JournalViews sends the location of
+    // the persistentIndirectionTable to the StateViews (although,
+    // at this point, it's abstracted out to being just "the location
+    // of the state")
+    //
+    // In order to update the indirection table, we do a
+    // Freeze -> SendFrozenLoc -> CleanUp loop.
+    //
+    //  * Freeze: JournalViews doesn't do anything other than mark
+    //      that this is the place where the freeze took place.
+    //      Meanwhile, the StateViews updates its frozen state to
+    //      its ephemeral state.
+    //
+    //  * SendFrozenLoc: StateViews sends a loc to JournalViews.
+    //      It promises that the frozen state is now saved at that
+    //      loc and will persist after crashing.
+    //
+    //  * CleanUp: JournalViews promises to StateViews that it has now
+    //      updated the superblock's pointer to the frozen location.
+    //      StateView is now able to clean out its old persistent state
+    //      and update it to its frozen state.
+
+    | SendPersistentLocOp(loc: Loc)
+    | FreezeOp
     | SendFrozenLocOp(loc: Loc)
     | CleanUpOp
+
+    // Crash / syncing stuff. Syncing stuff is all handled
+    // by JournalViews.
+
+    | CrashOp
     | PushSyncOp(ghost id: int)
     | PopSyncOp(ghost id: int)
 
